on tactics: - renamed deduce into ded - added clear in the definition of gen - renamed normalize* into norm* - redefined case_eq as coq_case_eq with intro at the end - added case_beq and case_nat_eq as particular case - added hyp as abbrev of assumption

Util/Relation/Iter.v
@@ -86,7 +86,7 @@ Proof.
 induction n; simpl; intros; unfold inclusion; intros.
 do 2 destruct H. destruct x0. left. auto.
 right. exists (S x0). intuition.
-deduce (IHn _ _ H). destruct H0. left. right. exact H0.
+ded (IHn _ _ H). destruct H0. left. right. exact H0.
 do 2 destruct H0. case (le_lt_dec x0 (S n)); intro.
 assert (x0 = S n). omega. subst x0. left. left. exact H1.
 right. exists x0. intuition.
@@ -128,116 +128,128 @@ Qed.
 
 (** Other definitions of iter_le, easier for induction *)
 
-Fixpoint iter_le2  n :=
-match n with 
-  |O => R
-  |S i => (R @ iter_le2 i)  U iter_le2 i 
+Fixpoint iter_le2 n :=
+  match n with 
+    | O => R
+    | S i => (R @ iter_le2 i) U iter_le2 i 
   end.
 
 Fixpoint iter_le_fast n :=
-match n with 
-  |O => R
-  |S i => let R':=iter_le_fast i in 
-  R' @ R' U R'
+  match n with 
+    | O => R
+    | S i => let R' := iter_le_fast i in R' @ R' U R'
   end.
 
 (** Equivalence between differents definitions *)
 
-Lemma iter_le_spec : forall n x y, iter_le n x y <-> 
-exists p, p <= n /\ iter p x y.
-intro;induction n.
-intros;simpl in *.
-split;intros. exists 0;split;auto with *.
-destruct H as [p];destruct H; assert(p=0);auto with *.
-subst;auto with *. 
-split;intros;simpl in *.
-unfold compose in H;destruct H.
-destruct H as [z]; exists (S n); split;auto with *.
-simpl;unfold compose;exists z;assumption.
+Lemma iter_le_spec : forall n x y,
+  iter_le n x y <-> exists p, p <= n /\ iter p x y.
 
-rewrite IHn in H;destruct H as [p]; exists p; intuition; auto with *.
+Proof.
+intro; induction n.
+intros; simpl in *.
+split; intros. exists 0; split; auto with *.
+destruct H as [p]; destruct H; assert(p=0); auto with *.
+subst; auto with *. 
+split; intros; simpl in *.
+unfold compose in H; destruct H.
+destruct H as [z]; exists (S n); split; auto with *.
+simpl; unfold compose; exists z; assumption.
 
-destruct H as [p];destruct H. destruct (le_lt_eq_dec p (S n) H).
-right; apply lt_n_Sm_le in l;rewrite IHn;exists p;auto with *.
-subst;left;unfold compose in H0;auto with *.
+rewrite IHn in H; destruct H as [p]; exists p; intuition; auto with *.
+
+destruct H as [p]; destruct H. destruct (le_lt_eq_dec p (S n) H).
+right; apply lt_n_Sm_le in l; rewrite IHn; exists p; auto with *.
+subst; left; unfold compose in H0; auto with *.
 Qed.
 
-Lemma iter_le2_spec : forall n x y, iter_le2 n x y <-> 
-exists p, p <= n /\ iter p x y.
+Lemma iter_le2_spec : forall n x y,
+  iter_le2 n x y <-> exists p, p <= n /\ iter p x y.
+
+Proof.
 intro. induction n.
-intros;simpl in *;split;intros. exists 0;split;auto with *.
-destruct H as [p];destruct H; assert(p=0);auto with *.
-subst;auto with *. 
-split;intros;simpl in *.
+intros; simpl in *; split; intros. exists 0; split; auto with *.
+destruct H as [p]; destruct H; assert(p=0); auto with *.
+subst; auto with *. 
+split; intros; simpl in *.
 
 unfold compose in H; destruct H.
-destruct H as [z];destruct H;rewrite IHn in H0;destruct H0 as [p];exists (S p).
- split;auto with *. simpl;unfold compose;exists z;intuition; auto with *.
+destruct H as [z]; destruct H; rewrite IHn in H0; destruct H0 as [p];
+  exists (S p).
+split; auto with *. simpl; unfold compose; exists z; intuition; auto with *.
 
-rewrite IHn in H;destruct H as [p]; exists p; intuition; auto with *.
+rewrite IHn in H; destruct H as [p]; exists p; intuition; auto with *.
 
-destruct H as [p];destruct H.
+destruct H as [p]; destruct H.
 destruct (le_lt_eq_dec p (S n) H).
-right; apply lt_n_Sm_le in l;rewrite IHn;exists p;auto with *.
-subst;left;unfold compose in H0;auto with *.
-simpl in H0;unfold compose in *;destruct H0 as [z];exists z.
-split;destruct H0;auto with *.
-rewrite IHn;exists n;auto.
+right; apply lt_n_Sm_le in l; rewrite IHn; exists p; auto with *.
+subst; left; unfold compose in H0; auto with *.
+simpl in H0; unfold compose in *; destruct H0 as [z]; exists z.
+split; destruct H0; auto with *.
+rewrite IHn; exists n; auto.
 Qed.
 
 
 Lemma iter_compose : forall p q, iter p @ iter q << iter (p+q+1).
+
 Proof.
 intros; induction p.
-assert (S(q) = q+1);auto with *.
-simpl;rewrite <- H;simpl;intuition.
-unfold inclusion;intros.
-simpl in H;repeat destruct H.
-simpl;unfold compose.
-exists x1;split;auto with *.
-unfold inclusion in IHp;eapply IHp.
-simpl;unfold compose.
-exists x0;split;auto with *.
+assert (S(q) = q+1); auto with *.
+simpl; rewrite <- H; simpl; intuition.
+unfold inclusion; intros.
+simpl in H; repeat destruct H.
+simpl; unfold compose.
+exists x1; split; auto with *.
+unfold inclusion in IHp; eapply IHp.
+simpl; unfold compose.
+exists x0; split; auto with *.
 Qed.
 
 Require Export log2.
 
-Lemma iter_le_fast_spec : forall n x y, iter_le_fast n x y <-> 
-exists p,(S p) <= exp2 n /\ iter p x y.
+Lemma iter_le_fast_spec : forall n x y,
+  iter_le_fast n x y <-> exists p,(S p) <= exp2 n /\ iter p x y.
+
+Proof.
 intro. induction n.
-intros;simpl in *;split;intros. exists 0;split;auto with *.
-destruct H as [p];destruct H; assert(p=0);auto with *.
-subst;auto with *. split;intros;simpl in *.
+intros; simpl in *; split; intros. exists 0; split; auto with *.
+destruct H as [p]; destruct H; assert(p=0); auto with *.
+subst; auto with *. split; intros; simpl in *.
 destruct H. 
-destruct H as [z];destruct H. rewrite IHn in H0;rewrite IHn in H.
-destruct H0 as [p];destruct H as [p'];destruct H0;destruct H.
+destruct H as [z]; destruct H. rewrite IHn in H0; rewrite IHn in H.
+destruct H0 as [p]; destruct H as [p']; destruct H0; destruct H.
 exists (p+p'+1). split. omega.
 assert ((iter p' @ iter p) x y). unfold compose; exists z; auto with *.
-assert (p+p'+1=p'+p+1);intuition.
-rewrite H4;apply iter_compose;auto with *.
-rewrite IHn in H;destruct H as [p];exists p;intuition.
-destruct H as [p]; destruct H;simpl in H.
+assert (p+p'+1=p'+p+1); intuition.
+rewrite H4; apply iter_compose; auto with *.
+rewrite IHn in H; destruct H as [p]; exists p; intuition.
+destruct H as [p]; destruct H; simpl in H.
 
 destruct (le_gt_dec (S p) (exp2 n)).
-right;rewrite IHn;exists p;split;auto with *.
+right; rewrite IHn; exists p; split; auto with *.
 assert(p = (exp2 n - 1) + (p - exp2 n) +1 ).
 omega.
-rewrite H1 in H0. deduce (iter_plus_1 _ _ _ _ H0).
-left;unfold compose in *; destruct H2 as [z];destruct H2.
-exists z;split; rewrite IHn.
-exists (exp2 n -1); intuition;omega.
-exists (p -exp2 n); intuition;omega. 
+rewrite H1 in H0. ded (iter_plus_1 _ _ _ _ H0).
+left; unfold compose in *; destruct H2 as [z]; destruct H2.
+exists z; split; rewrite IHn.
+exists (exp2 n -1); intuition; omega.
+exists (p -exp2 n); intuition; omega. 
 Qed.
 
 
 Lemma iter_le_same : forall n x y, iter_le2 n x y <-> iter_le n x y.
+
 Proof.
-intros;rewrite iter_le_spec; rewrite iter_le2_spec; tauto.
+intros; rewrite iter_le_spec; rewrite iter_le2_spec; tauto.
 Qed.
-Lemma iter_le_fast_exp2_same : forall n x y, iter_le_fast n x y <-> iter_le ((exp2 n)-1) x y.
-intros;rewrite iter_le_spec; rewrite iter_le_fast_spec.
-split;intro;destruct H as [p];exists p; intuition.
-deduce (exp2_pos n);omega.
+
+Lemma iter_le_fast_exp2_same : forall n x y,
+  iter_le_fast n x y <-> iter_le ((exp2 n)-1) x y.
+
+Proof.
+intros; rewrite iter_le_spec; rewrite iter_le_fast_spec.
+split; intro; destruct H as [p]; exists p; intuition.
+ded (exp2_pos n); omega.
 Qed.
 
 (***********************************************************************)
@@ -248,7 +260,7 @@ Lemma iter_path : forall n x y,
 
 Proof.
 induction n; simpl; intros. exists (@nil A). intuition.
-do 2 destruct H. deduce (IHn _ _ H0). do 2 destruct H1. subst n.
+do 2 destruct H. ded (IHn _ _ H0). do 2 destruct H1. subst n.
 exists (x0 :: x1). simpl. intuition.
 Qed.
 
@@ -258,29 +270,29 @@ Proof.
 induction l; simpl; intros. exact H. exists a. intuition.
 Qed.
 
-Lemma bound_path_iter_le : forall n  x y, bound_path R n x y -> iter_le n x y.
+Lemma bound_path_iter_le : forall n x y, bound_path R n x y -> iter_le n x y.
+
 Proof.
-intro;induction n;intros; simpl in *.
-inversion H;subst;destruct l;simpl in *; auto with *;inversion H0.
-generalize (bound_path_Sn_n_or_Rn H);intros; destruct H0.
-simpl in *;right; apply IHn; auto with *.
-destruct H0 as [z];destruct H0;deduce (IHn _ _ H1).
-simpl;rewrite iter_le_spec in *;destruct H2 as [p];destruct H2.
+intro; induction n; intros; simpl in *.
+inversion H; subst; destruct l; simpl in *; auto with *; inversion H0.
+generalize (bound_path_Sn_n_or_Rn H); intros; destruct H0.
+simpl in *; right; apply IHn; auto with *.
+destruct H0 as [z]; destruct H0; ded (IHn _ _ H1).
+simpl; rewrite iter_le_spec in *; destruct H2 as [p]; destruct H2.
 destruct (le_lt_eq_dec p n H2).
-right;rewrite iter_le_spec;exists (S p);intuition.
-simpl;unfold compose;exists z;intuition.
-left;subst;unfold compose;exists z;intuition.
+right; rewrite iter_le_spec; exists (S p); intuition.
+simpl; unfold compose; exists z; intuition.
+left; subst; unfold compose; exists z; intuition.
 Qed.
 
 Lemma iter_le_bound_path : forall n x y, iter_le n x y -> bound_path R n x y .
+
 Proof.
 intros.
-rewrite iter_le_spec in H;destruct H as [j];destruct H.
-deduce (iter_path _ _ _ H0);destruct H1 as [l];destruct H1.
-eapply bp_intro;try eassumption;auto;subst;assumption.
+rewrite iter_le_spec in H; destruct H as [j]; destruct H.
+ded (iter_path _ _ _ H0); destruct H1 as [l]; destruct H1.
+eapply bp_intro; try eassumption; auto; subst; assumption.
 Qed.
-
-
 
 End S.
 
