Util/Relation/Cycle.v
@@ -7,7 +7,7 @@ See the COPYRIGHTS and LICENSE files.
 cycles
 *)
 
-(* $Id: Cycle.v,v 1.7 2007-02-23 14:20:53 stephaneleroux Exp $ *)
+(* $Id: Cycle.v,v 1.8 2008-05-14 12:26:55 blanqui Exp $ *)
 
 Set Implicit Arguments.
 
@@ -28,8 +28,8 @@ Lemma path_cycle : forall x y l, is_path R x y l -> In x l ->
   exists m, exists p, l = m ++ x :: p /\ cycle x m.
 
 Proof.
-intros. deduce (in_elim H0). do 2 destruct H1. subst l.
-deduce (path_app_elim H). destruct H1.
+intros. ded (in_elim H0). do 2 destruct H1. subst l.
+ded (path_app_elim H). destruct H1.
 exists x0. exists x1. intuition.
 Qed.
 
@@ -45,22 +45,23 @@ Lemma cycle_min_intro : forall x l, cycle x l ->
     x :: l = m ++ y :: p ++ q /\ cycle_min y p.
 
 Proof.
-intros. unfold cycle_min. deduce (repeat_free_intro eq_dec (x::l)). decomp H0.
+intros. unfold cycle_min. ded (repeat_free_intro eq_dec (x::l)). decomp H0.
 (* repeat_free (x::l) *)
 exists (@nil A). exists x. exists l. exists (@nil A). rewrite <- app_nil_end.
 simpl in H1. intuition.
 (* x::l = x0++x1::x2 *)
-rewrite H1. deduce (in_elim H4). decomp H0. rewrite H5.
+rewrite H1. ded (in_elim H4). decomp H0. rewrite H5.
 exists x3. exists x1. exists x4. exists (x1::x2). rewrite app_ass. simpl.
-rewrite H5 in H2. deduce (repeat_free_app_elim H2). simpl in H0. decomp H0. intuition.
+rewrite H5 in H2. ded (repeat_free_app_elim H2). simpl in H0. decomp H0.
+intuition.
 (* cycle x1 x4 *)
 destruct x0. contradiction. injection H1; intros. subst a.
 unfold cycle in H. destruct x3; injection H5; intros.
 (* x3=nil *)
-subst x1. subst x4. rewrite H0 in H. deduce (path_app_elim H). intuition.
+subst x1. subst x4. rewrite H0 in H. ded (path_app_elim H). intuition.
 (* x3=x::x3 *)
 subst a. subst x0. rewrite app_ass in H0. simpl in H0. rewrite H0 in H.
-deduce (path_app_elim H). destruct H7. deduce (path_app_elim H10). intuition.
+ded (path_app_elim H). destruct H7. ded (path_app_elim H10). intuition.
 Qed.
 
 End S.
